kremlib/Spec.Loops.fst
@@ -32,3 +32,13 @@ let rec seq_map2 #a #b #c f s s' =
 
 val repeat_spec: #a:Type -> n:nat -> (f: a -> Tot a) -> a -> Tot a (decreases n)
 let rec repeat_spec #a n f x = if n = 0 then x else repeat_spec (n-1) f (f x)
+
+val lemma_repeat: #a:Type -> n:nat{n > 0} -> f:( a -> Tot a) -> x:a -> Lemma
+  (repeat_spec n f x == f (repeat_spec (n-1) f x))
+let rec lemma_repeat #a n f x =
+  if n = 1 then ()
+  else lemma_repeat (n-1) f (f x)
+
+val lemma_repeat_0: #a:Type -> n:nat{n = 0} -> f:( a -> Tot a) -> x:a -> Lemma
+  (repeat_spec n f x == x)
+let rec lemma_repeat_0 #a n f x = ()
